Regenerate

TestModels/Streaming/src/SimpleStreamingImpl.dfy
@@ -1,126 +1,49 @@
-
-
+// Copyright Amazon.com Inc. or its affiliates. All Rights Reserved.
+// SPDX-License-Identifier: Apache-2.0
+// Do not modify this file. This file is machine generated, and any changes to it will be overwritten.
 include "../Model/SimpleStreamingTypes.dfy"
+module SimpleStreamingImpl refines AbstractSimpleStreamingOperations {
+  datatype Config = Config
+  type InternalConfig = Config
+  predicate ValidInternalConfig?(config: InternalConfig)
+  {true}
+  function ModifiesInternalConfig(config: InternalConfig): set<object>
+  {{}}
+  predicate CountBitsEnsuresPublicly(input: CountBitsInput , output: Result<CountBitsOutput, Error>)
+  {true}
 
-module SimpleStreamingImpl refines AbstractSimpleStreamingOperations  {
-    datatype Config = Config
-    type InternalConfig = Config
-    predicate ValidInternalConfig?(config: InternalConfig)
-    {true}
-    function ModifiesInternalConfig(config: InternalConfig) : set<object>
-    {{}}
-    predicate GetStringEnsuresPublicly(input: GetStringInput, output: Result<GetStringOutput, Error>) {
-        true
-    }
-    predicate GetStringKnownValueEnsuresPublicly(input: GetStringInput, output: Result<GetStringOutput, Error>) {
-        true
-    }
-    predicate GetStringUTF8EnsuresPublicly(input: GetStringInput, output: Result<GetStringOutput, Error>) {
-        true
-    }
-    method GetString ( config: InternalConfig,  input: GetStringInput )
-    returns (output: Result<GetStringOutput, Error>) {
-        var res := GetStringOutput(value := input.value);
-        return Success(res);
-    }
-    method GetStringKnownValue ( config: InternalConfig,  input: GetStringInput )
-    returns (output: Result<GetStringOutput, Error>) {
-        expect input.value.Some?;
-        expect input.value.value == "TEST_SIMPLE_STRING_KNOWN_VALUE"; // This is done so as to assert that polymorph layer is doing one way conversion right as well.
-        var res := GetStringOutput(value := input.value);
-        return Success(res);
-    }
-    method GetStringUTF8 ( config: InternalConfig,  input: GetStringInput )
-    returns (output: Result<GetStringOutput, Error>) {
-        expect input.value.Some?;
-        var res := GetStringOutput(value := input.value);
-        return Success(res);
-    }
-}
 
-module Foo {
 
-  type Error
+  method CountBits ( config: InternalConfig , input: CountBitsInput )
+    returns (output: Result<CountBitsOutput, Error>)
 
-  // GENERATED
+  {
+    expect false, "...that you'll fill this in";
+  }
 
-  // TODO: Check Smithy spec about when response is received
-  // TODO: Actions pretty much always have to return Results/Outcomes
 
-  method StreamingBlobInput(input: StreamingBlobRequest, onResult: SingleUseAction<Result<StreamingBlobResponse, Error>, ()>) 
-    returns (onInputData: Action<Option<bytes>, ()>)
-    ensures ConsumesTerminated(onInputData)
+  predicate BinaryOfEnsuresPublicly(input: BinaryOfInput , output: Result<BinaryOfOutput, Error>)
+  {true}
 
-  datatype StreamingBlobOutputEvent =
-    | StreamingBlobOutputData(data: bytes)
-    | StreamingBlobOutputSuccess(response: StreamingBlobResponse)
-    | StreamingBlobOutputFailure(error: Error)
 
-  method StreamingBlobOutput(input: StreamingBlobRequest, onResultEvent: Action<StreamingBlobOutputEvent, ()>) 
-    // TODO: needs a requires clause about sequences of events the callback will consume
 
-  method StreamingBlobInputAndOutput(input: StreamingBlobRequest, onResultEvent: Action<StreamingBlobOutputEvent, ()>) 
-    returns (onInputData: Action<Option<bytes>, ()>)
-    ensures ConsumesTerminated(onInputData)
-    // TODO: needs a requires clause about sequences of events the callback will consume
-}
+  method BinaryOf ( config: InternalConfig , input: BinaryOfInput )
+    returns (output: Result<BinaryOfOutput, Error>)
 
-// Synchronous-only style
-// TODO: Show how to wrap this interface around asynchronous AWS service calls?
-module DafnyStyle {
+  {
+    expect false, "...that you'll fill this in";
+  }
 
-  import opened StdLib  
 
-  datatype StreamingBlobRequest = StreamingBlobRequest()
-  datatype StreamingBlobResponse = StreamingBlobResponse()
+  predicate ChunksEnsuresPublicly(input: ChunksInput , output: Result<ChunksOutput, Error>)
+  {true}
 
-  type Error
 
-  // TODO: Spec on when sink will be called vs. onData
-  method StreamingBlobInput(input: StreamingBlobRequest) 
-    returns (onInputData: Action<Option<bytes>, 
-                                 Option<Result<StreamingBlobResponse, Error>>>)
-    ensures ConsumesTerminated(onInputData)
-    // TODO: With @requiresLength, ensures something about |flattened(produced(onInputData))|
 
-  datatype StreamingBlobOutputEvent =
-    | StreamingBlobOutputData(data: bytes)
-    | StreamingBlobOutputSuccess(response: StreamingBlobResponse)
-    | StreamingBlobOutputFailure(error: Error)
+  method Chunks ( config: InternalConfig , input: ChunksInput )
+    returns (output: Result<ChunksOutput, Error>)
 
-  method StreamingBlobOutput(input: StreamingBlobRequest) 
-    returns (resultIter: Action<(), StreamingBlobOutputEvent>)
-    ensures ConsumesAnything(resultIter)
-    // TODO: ensures Enumerator(resultIter), or a variant of it that can error
-
-  method StreamingBlobInputAndOutput(input: StreamingBlobRequest) 
-    // Two different ways to implement this around e.g. S3:
-    // * Send input, block on next output event
-    // * Send input, return 
-    returns (onInputData: Action<Option<bytes>, StreamingBlobOutputEvent>)
-    ensures ConsumesTerminated(onInputData)
-}
-
-module Bar {
-  import opened StdLib
-  import opened Foo
-
-  method Consumer() {
-
-    var input := StreamingBlobRequest();
-
-    var result: StreamingBlobResponse;
-    // TODO: store in result
-    var onResult: SingleUseAction<Result<StreamingBlobResponse, Error>, ()>;
-    
-    var onInputData := StreamingBlobInput(input, onResult);
-    Call(onInputData, Some([1, 2]));
-    Call(onInputData, Some([3, 4, 5]));
-    Call(onInputData, None);
-
-    // result now has the result
-    // TODO: how to express that specification?
-    // TODO: Could have
-
+  {
+    expect false, "...that you'll fill this in";
   }
 }
